RakeMap: moved rem lemmas into Rake

RakeMap.lean
@@ -1,8 +1,8 @@
 import Rake
 
 /--
-A RakeMap is a Rake that provides a 1-to-1 mapping between
-the rake and a set of numbers with some property. -/
+A RakeMap provides a 1-to-1 mapping between its rake
+and a set of numbers with some property. -/
 structure RakeMap (pred: Nat → Prop) where
   rake : Rake
   hbij : ∀ n, pred n ↔ ∃ m, rake.term m = n
@@ -33,48 +33,22 @@ def rm_ge2 : RakeMap (λn => 2≤n) := {
     · show (∃ m, 2 + m = n) → 2 ≤ n
       intro hm; obtain ⟨m,hm⟩ := hm; rw[←hm]; simp }
 
-section rem_lemmas
-
-  -- now it's more complicated. first we partition each sequence
-  -- then we remove the sequences that are multiples of a prime
-  -- how do we know:
-  --   - we dropped the multiples?
-  --     - partition step keeps same terms
-  --     - but now every sequence either ALWAYS or NEVER produces multiples of p
-  --     - we can tell the difference, and only drop the ones that always produce multiples
-  --   - we know we kept everything else because it's a straight filter operation.
-
-
-  variable (rm: RakeMap prop) (p n: Nat) {hp: 0<p}
-
-  lemma rem_drop -- rem drops multiples of p
-    : p∣n → ¬(∃m, (rm.rake.rem p).sort.val.term m = n) := by
-    sorry
-
-  lemma rem_keep -- rem keeps non-multiples of p
-    : ¬(p∣n) ∧ (∃pm, rm.rake.term pm = n) → (∃m, (rm.rake.rem p).sort.val.term m = n) := by
-    sorry
-
-  lemma rem_same -- rem introduces no new terms
-    : (∃m, (rm.rake.rem p).sort.val.term m = n) → (∃pm, rm.rake.term pm = n) := by
-    sorry
-
-end rem_lemmas
-
 -- operations on RakeMap -------------------------------------------------------
 
--- def RakeMap.sort (rm: RakeMap prop) : RakeMap prop // }
-
-def rem (rm : RakeMap prop) (p: Nat)
-  : RakeMap (λ n => prop n ∧ ¬(p∣n)) :=
-  let rake := (rm.rake.rem p).sort
-  let proof := by
-    intro n; symm
-    let hm : Prop := (∃m, rake.val.term m = n)
-    let hpm : Prop := (∃pm, rm.rake.term pm = n )
-    have : prop n ↔ hpm := rm.hbij n
-    have : p∣n → ¬hm := rem_drop rm p n
-    have : ¬p∣n ∧ hpm → hm := rem_keep rm p n
-    have : hm → hpm := rem_same rm p n
-    by_cases p∣n; all_goals aesop
-  { rake := rake, hbij := proof, hord := rake.prop }
+def rem (rm : RakeMap prop) (x: Nat)
+  : RakeMap (λ n => prop n ∧ ¬(x∣n)) :=
+  let r₀ := rm.rake
+  let r₁ := r₀.rem x
+  have hbij₀ : ∀ n, prop n ∧ ¬(x∣n) ↔ ∃ m, r₁.term m = n := by
+    intro n
+    have hb := rm.hbij
+    have hd := r₀.rem_drop x n
+    have hk := r₀.rem_keep x n
+    have hs := r₀.rem_same x n
+    apply Iff.intro; by_cases x∣n; all_goals aesop
+  let r₂ := r₁.sort
+  let hbij₂ : ∀ n, prop n ∧ ¬(x∣n) ↔ ∃ m, r₂.val.term m = n := by
+    intro n
+    have hs := r₁.sort_term_iff_term n
+    apply Iff.intro; all_goals aesop
+  { rake := r₂, hbij := hbij₂, hord := r₂.prop }
